examples/Stack/go.sh
@@ -2,10 +2,13 @@
 # && make -C../../lib/coq -j3 \
 # && make -C ../../lib/stdlib \
 
+# && make -f ../Makefile.dev ML=`pwd`/Stack.ml
+
 make -C ../.. install \
 && make -f ../Makefile.dev _CoqProject \
-&& make -f ../Makefile.dev
-FILE=`basename \`pwd\``
+&& make -f ../Makefile.dev ML=`pwd`/StackSized.ml
+# FILE=`basename \`pwd\``
+FILE=StackSized
 coqide -async-proofs off -async-proofs-command-error-resilience off ${FILE}_ml.v ${FILE}_proof.v &
 
 
